theories/DeFi.v
@@ -1,0 +1,37 @@
+(* A theory of AMMs and DeFi, embedded in Coq 
+    This is an outline of future work that leverages morphisms, bisimulations,
+    and meta specifications to create a theory of AMMs and DeFi, embedded in Coq.
+*)
+
+From Coq Require Import Basics.
+From Coq Require Import List.
+From Coq Require Import String.
+From Coq Require Import Sets.Ensembles.
+From Coq Require Import ZArith.
+From Coq Require Import ProofIrrelevance.
+From Coq Require Import Permutation.
+From Coq Require Import FunctionalExtensionality.
+From ConCert.Execution Require Import ChainedList.
+From ConCert.Execution Require Import Blockchain.
+From ConCert.Execution Require Import Serializable.
+From ConCert.Execution Require Import ResultMonad.
+From FinCert.Meta Require Import ContractMorphisms.
+From FinCert.Meta Require Import ContractSystems.
+From FinCert.Meta Require Import Bisimulation.
+
+Import ListNotations.
+
+(*
+
+Define **desirable economic properties**
+
+- start with some model of "what an AMM is" -- can be in terms of one contract, or drawing on abstract specifications, e.g. the token specifications
+
+- not only do we have a specification (& metaspec) of a specific AMM, but we can 
+    **further abstract** from there to prove properties of AMMs
+
+- you need contraction over the link graph to really do this ... this is very hard.
+
+USE THESE TO STUDY DEXTER2 FROM BEFORE
+
+*)
