theories/README.md
@@ -1,3 +1,61 @@
 # Theories 
 
-A subdirectory for theories, *e.g.* a theory of DeFi, which can inform contract specification and verification.
+This subdirectory contains the theory of smart contracts. We study the 
+computational structure of smart contracts in order to support reasoning
+about its meta properties. These include 
+upgradeability properties, as well as properties of multiple contracts taken
+as a whole.
+
+The first, fundamental notion we introduce is that of a morphism of contracts.
+
+## Contract Morphisms
+Contract morphisms are functions between smart contracts that relate their 
+structureal and computational properties.
+Because contracts in ConCert are given by a pair of functions, 
+`init` and `receive`, a contract morphism between contracts `C1` and `C2` is 
+a pair of functions between each contract's `init` and `receive` functions,
+respectively.
+
+```
+          inputs (receive C1) ->  inputs (receive C2)
+                |                       |                  
+                v                       v                  
+          outputs (receive C1) -> outputs (receive C1)              
+```
+
+A contract morphism can be used in proof and specification of a smart
+contract. They can:
+-   specify upgrades (see [the upgrade specification example](../examples/ContractMorphisms/specifyUpgrade/))
+-   transport Hoare properties of partial correctness (see [Hoare example](../examples/ContractMorphisms/transportHoare/))
+-   be used to prove [one contract backwards compatible with another](../examples/ContractMorphisms/backwardsCompatible/)
+-   deconstruct a [contract's upgradeability properties](../examples/ContractMorphisms/upgradeable/), separating it into its immutable and mutable parts.
+
+In the [contract morphisms module](ContractMorphisms.v) we also introduce a generic technique to use a contract morphism with ConCert's custom tactic, `contract_induction`.
+
+If two contract morphisms `f : C1 -> C2` and `g : C2 -> C1` compose each way to the identity morphism, we say that `C1` and `C2` are *isomorphic*.
+This means that `C1` and `C2` are isomorphic, or equivalent, in some sense.
+Of course, a bisimulation is the most influential notion of equivalence between processes.
+
+## Bisimulation
+
+A bisimulation is an isomorhpism of system traces. 
+To establish a bisimulation of contracts `C1` and `C2`, we need a function `st_morph` between their respective storage types and a function between contract steps (how a contract moves forward) such that:
+1. `st_morph` sends initial states of `C1` to initial states of `C2`, and 
+1. if `C1` can step from states `st1` to `st2`, then `C2` can step from `(st_morph st1)` to `(st_morph st2)`
+
+Given any execution trace of `C1`, this gives us a corresponding trace of `C2`. If `st_morph` has an inverse that satisfies the properties above, then this gives us a *bisimulation* between contracts `C1` and `C2`.
+This means that execution traces are in one-to-one correspondence under these *morphisms of contract traces*.
+
+An isomorphism of contracts produces a bisimulation of their traces.
+
+This is formalized in the [bisimulation module](Bisimulation.v).
+
+## Considering Contract Systems
+
+In practice, when writing or verifying a smart contract, we care about the behavior of multiple contracts simultaneously. In the [contract systems module](ContractSystems.v), we define a data structure for systems of contracts that lets us consider some contracts "nested within" others.
+
+Like for contracts, systems of contracts have a notion of system morphism and system bisimulation.
+
+## Future Work: A Formalized Theory of AMMs and DeFi
+
+The theoretical tools of metaspecification, contract morphisms, contract systems, and bisimulation, lay the foundation for a formalized theory of AMMs and DeFi in ConCert, which we outline in the [DeFi module](DeFi.v).
